verif/dlinklist.v
@@ -67,51 +67,53 @@ Definition ___compcert_va_float64 : ident := 26%positive.
 Definition ___compcert_va_int32 : ident := 24%positive.
 Definition ___compcert_va_int64 : ident := 25%positive.
 Definition _begin : ident := 66%positive.
-Definition _delete : ident := 81%positive.
+Definition _delete : ident := 83%positive.
 Definition _end : ident := 67%positive.
 Definition _freeN : ident := 61%positive.
-Definition _get_size : ident := 70%positive.
+Definition _get_size : ident := 72%positive.
 Definition _head : ident := 6%positive.
-Definition _insert : ident := 80%positive.
-Definition _k : ident := 85%positive.
+Definition _insert : ident := 82%positive.
+Definition _k : ident := 87%positive.
 Definition _l : ident := 62%positive.
-Definition _l1 : ident := 82%positive.
-Definition _l2 : ident := 83%positive.
+Definition _l1 : ident := 84%positive.
+Definition _l2 : ident := 85%positive.
 Definition _list : ident := 8%positive.
 Definition _list_free : ident := 65%positive.
 Definition _list_new : ident := 63%positive.
-Definition _main : ident := 87%positive.
+Definition _main : ident := 89%positive.
 Definition _mallocN : ident := 60%positive.
-Definition _merge : ident := 84%positive.
-Definition _move : ident := 79%positive.
-Definition _nd : ident := 72%positive.
+Definition _merge : ident := 86%positive.
+Definition _move : ident := 81%positive.
+Definition _nd : ident := 74%positive.
 Definition _next : ident := 4%positive.
 Definition _node : ident := 2%positive.
-Definition _pop_back : ident := 75%positive.
-Definition _pop_front : ident := 77%positive.
-Definition _pos : ident := 78%positive.
+Definition _p : ident := 70%positive.
+Definition _pop_back : ident := 77%positive.
+Definition _pop_front : ident := 79%positive.
+Definition _pos : ident := 80%positive.
 Definition _prev : ident := 3%positive.
-Definition _push_back : ident := 73%positive.
-Definition _push_front : ident := 76%positive.
+Definition _push_back : ident := 75%positive.
+Definition _push_front : ident := 78%positive.
 Definition _rbegin : ident := 68%positive.
 Definition _rend : ident := 69%positive.
-Definition _res : ident := 74%positive.
+Definition _res : ident := 76%positive.
+Definition _rnext : ident := 71%positive.
 Definition _size : ident := 5%positive.
-Definition _split_K : ident := 86%positive.
+Definition _split_K : ident := 88%positive.
 Definition _tail : ident := 7%positive.
 Definition _tmp : ident := 64%positive.
-Definition _v : ident := 71%positive.
+Definition _v : ident := 73%positive.
 Definition _val : ident := 1%positive.
-Definition _t'1 : ident := 88%positive.
-Definition _t'10 : ident := 97%positive.
-Definition _t'2 : ident := 89%positive.
-Definition _t'3 : ident := 90%positive.
-Definition _t'4 : ident := 91%positive.
-Definition _t'5 : ident := 92%positive.
-Definition _t'6 : ident := 93%positive.
-Definition _t'7 : ident := 94%positive.
-Definition _t'8 : ident := 95%positive.
-Definition _t'9 : ident := 96%positive.
+Definition _t'1 : ident := 90%positive.
+Definition _t'10 : ident := 99%positive.
+Definition _t'2 : ident := 91%positive.
+Definition _t'3 : ident := 92%positive.
+Definition _t'4 : ident := 93%positive.
+Definition _t'5 : ident := 94%positive.
+Definition _t'6 : ident := 95%positive.
+Definition _t'7 : ident := 96%positive.
+Definition _t'8 : ident := 97%positive.
+Definition _t'9 : ident := 98%positive.
 
 Definition f_list_new := {|
   fn_return := (tptr (Tstruct _list noattr));
@@ -264,6 +266,36 @@ Definition f_rend := {|
     (Efield
       (Ederef (Etempvar _l (tptr (Tstruct _list noattr)))
         (Tstruct _list noattr)) _head (tptr (Tstruct _node noattr))))
+  (Sreturn (Some (Etempvar _t'1 (tptr (Tstruct _node noattr))))))
+|}.
+
+Definition f_next := {|
+  fn_return := (tptr (Tstruct _node noattr));
+  fn_callconv := cc_default;
+  fn_params := ((_p, (tptr (Tstruct _node noattr))) :: nil);
+  fn_vars := nil;
+  fn_temps := ((_t'1, (tptr (Tstruct _node noattr))) :: nil);
+  fn_body :=
+(Ssequence
+  (Sset _t'1
+    (Efield
+      (Ederef (Etempvar _p (tptr (Tstruct _node noattr)))
+        (Tstruct _node noattr)) _next (tptr (Tstruct _node noattr))))
+  (Sreturn (Some (Etempvar _t'1 (tptr (Tstruct _node noattr))))))
+|}.
+
+Definition f_rnext := {|
+  fn_return := (tptr (Tstruct _node noattr));
+  fn_callconv := cc_default;
+  fn_params := ((_p, (tptr (Tstruct _node noattr))) :: nil);
+  fn_vars := nil;
+  fn_temps := ((_t'1, (tptr (Tstruct _node noattr))) :: nil);
+  fn_body :=
+(Ssequence
+  (Sset _t'1
+    (Efield
+      (Ederef (Etempvar _p (tptr (Tstruct _node noattr)))
+        (Tstruct _node noattr)) _prev (tptr (Tstruct _node noattr))))
   (Sreturn (Some (Etempvar _t'1 (tptr (Tstruct _node noattr))))))
 |}.
 
@@ -1422,6 +1454,7 @@ Definition global_definitions : list (ident * globdef fundef type) :=
  (_list_free, Gfun(Internal f_list_free)) ::
  (_begin, Gfun(Internal f_begin)) :: (_end, Gfun(Internal f_end)) ::
  (_rbegin, Gfun(Internal f_rbegin)) :: (_rend, Gfun(Internal f_rend)) ::
+ (_next, Gfun(Internal f_next)) :: (_rnext, Gfun(Internal f_rnext)) ::
  (_get_size, Gfun(Internal f_get_size)) ::
  (_push_back, Gfun(Internal f_push_back)) ::
  (_pop_back, Gfun(Internal f_pop_back)) ::
@@ -1433,9 +1466,9 @@ Definition global_definitions : list (ident * globdef fundef type) :=
 
 Definition public_idents : list ident :=
 (_split_K :: _merge :: _delete :: _insert :: _move :: _pop_front ::
- _push_front :: _pop_back :: _push_back :: _get_size :: _rend :: _rbegin ::
- _end :: _begin :: _list_free :: _list_new :: _freeN :: _mallocN ::
- ___builtin_debug :: ___builtin_write32_reversed ::
+ _push_front :: _pop_back :: _push_back :: _get_size :: _rnext :: _next ::
+ _rend :: _rbegin :: _end :: _begin :: _list_free :: _list_new :: _freeN ::
+ _mallocN :: ___builtin_debug :: ___builtin_write32_reversed ::
  ___builtin_write16_reversed :: ___builtin_read32_reversed ::
  ___builtin_read16_reversed :: ___builtin_fnmsub :: ___builtin_fnmadd ::
  ___builtin_fmsub :: ___builtin_fmadd :: ___builtin_fmin ::
